[1021. Remove Outermost Parentheses](https://leetcode.com/problems/remove-outermost-parentheses/)

A valid parentheses string is either empty `""`, `"(" + A + ")"`, or `A + B`, where `A` and `B` are valid parentheses strings, and `+` represents string concatenation.

* For example, `""`, `"()"`, `"(())()"`, and `"(()(()))"` are all valid parentheses strings.

A valid parentheses string `s` is primitive if it is nonempty, and there does not exist a way to split it into `s = A + B`, with `A` and `B` nonempty valid parentheses strings.

Given a valid parentheses string `s`, consider its primitive decomposition: `s = P<sub>1</sub> + P<sub>2</sub> + ... + P<sub>k</sub>`, where `P<sub>i</sub>` are primitive valid parentheses strings.

Return `s` *after removing the outermost parentheses of every primitive string in the primitive decomposition of* `s`.

**Example 1:**

<pre><strong>Input:</strong> s = "(()())(())"
<strong>Output:</strong> "()()()"
<strong>Explanation:</strong> 
The input string is "(()())(())", with primitive decomposition "(()())" + "(())".
After removing outer parentheses of each part, this is "()()" + "()" = "()()()".
</pre>

**Example 2:**

<pre><strong>Input:</strong> s = "(()())(())(()(()))"
<strong>Output:</strong> "()()()()(())"
<strong>Explanation:</strong> 
The input string is "(()())(())(()(()))", with primitive decomposition "(()())" + "(())" + "(()(()))".
After removing outer parentheses of each part, this is "()()" + "()" + "()(())" = "()()()()(())".
</pre>

**Example 3:**

<pre><strong>Input:</strong> s = "()()"
<strong>Output:</strong> ""
<strong>Explanation:</strong> 
The input string is "()()", with primitive decomposition "()" + "()".
After removing outer parentheses of each part, this is "" + "" = "".
</pre>

**Constraints:**

* `1 <= s.length <= 10<sup>5</sup>`
* `s[i]` is either `'('` or `')'`.
* `s` is a valid parentheses string.

**Solution:**

```
class Solution {
    func removeOuterParentheses(_ s: String) -> String {
        var stack = ""
        var ans = ""
        var bag = ""
        for c in s {
            if c == ")" && stack.last == "(" {
                stack.popLast()
            } else {
                stack.append(c)
            }
            if stack.isEmpty {
                bag.removeFirst()
                ans.append(bag)
                bag = ""
            } else {
                bag.append(c)
            }
        }
        return ans
    }
}
```
